examples/pseudo_bool/array/mcisProgScript.sml
@@ -1,0 +1,655 @@
+(*
+  MCIS (connected) encode and checker
+*)
+open preamble basis pbc_normaliseTheory npbc_parseProgTheory mcisTheory graph_basicTheory;
+
+val _ = new_theory "mcisProg"
+
+val _ = translation_extends"npbc_parseProg";
+
+val xlet_autop = xlet_auto >- (TRY( xcon) >> xsimpl)
+
+(* parsing
+  TODO: blanks already translated using the copy in pb_parse
+  val _ = translate graph_basicTheory.blanks_def; *)
+val _ = translate graph_basicTheory.tokenize_num_def;
+
+val _ = translate parse_num_list_def;
+val _ = translate parse_edges_def;
+val _ = translate parse_lad_toks_def;
+
+Theorem check_good_edges_inner_thm:
+  check_good_edges_inner u v es ⇔
+  case lookup u es of NONE => F | SOME edges => MEMBER v edges
+Proof
+  fs[check_good_edges_inner_def,MEMBER_INTRO]>>
+  metis_tac[]
+QED
+
+val _ = translate check_good_edges_inner_thm;
+
+val _ = translate (check_good_edges_def |> SIMP_RULE std_ss [GSYM check_good_edges_inner_def]);
+val _ = translate check_good_graph_def;
+
+val tokenize_num_v_thm = theorem "tokenize_num_v_thm";
+
+val b_inputAllTokensFrom_spec_specialize =
+  b_inputAllTokensFrom_spec
+  |> Q.GEN `f` |> Q.SPEC`blanks`
+  |> Q.GEN `fv` |> Q.SPEC`blanks_v`
+  |> Q.GEN `g` |> Q.ISPEC`tokenize_num`
+  |> Q.GEN `gv` |> Q.ISPEC`tokenize_num_v`
+  |> Q.GEN `a` |> Q.ISPEC`SUM_TYPE STRING_TYPE NUM`
+  |> REWRITE_RULE [blanks_v_thm,tokenize_num_v_thm] ;
+
+val noparse_string_def = Define`
+  noparse_string f s = concat[strlit"c Input file: ";f;strlit" unable to parse in format: "; s;strlit"\n"]`;
+
+val r = translate noparse_string_def;
+
+val parse_lad = (append_prog o process_topdecs) `
+  fun parse_lad f =
+  (case TextIO.b_inputAllTokensFrom f blanks tokenize_num of
+    None => Inl (notfound_string f)
+  | Some lines =>
+  (case parse_lad_toks lines of
+    None => Inl (noparse_string f "LAD")
+  | Some x =>
+    if check_good_graph x then
+      Inr x
+    else Inl ("c Input graph " ^ f ^ " fails undirectedness check\n")))`
+
+Theorem blanks_eq[simp]:
+  graph_basic$blanks = pb_parse$blanks
+Proof
+  rw[FUN_EQ_THM]>>
+  simp[pb_parseTheory.blanks_def,blanks_def]
+QED
+
+Overload "graph_TYPE" = ``PAIR_TYPE NUM (SPTREE_SPT_TYPE (LIST_TYPE NUM))``;
+
+(* get_graph *)
+Definition get_graph_def:
+  get_graph fs f =
+  if inFS_fname fs f then
+    case parse_lad (all_lines fs f) of
+      NONE => NONE
+    | SOME g =>
+      if good_graph g then
+        SOME g
+      else NONE
+  else NONE
+End
+
+Theorem parse_lad_spec:
+  STRING_TYPE f fv ∧
+  validArg f ∧
+  hasFreeFD fs
+  ⇒
+  app (p:'ffi ffi_proj) ^(fetch_v"parse_lad"(get_ml_prog_state()))
+    [fv]
+    (STDIO fs)
+    (POSTv v.
+    & (∃err. SUM_TYPE STRING_TYPE graph_TYPE
+      (case get_graph fs f of
+        NONE => INL err
+      | SOME res => INR res) v) * STDIO fs)
+Proof
+  rw[]>>
+  xcf"parse_lad"(get_ml_prog_state())>>
+  reverse (Cases_on `STD_streams fs`) >- (fs [TextIOProofTheory.STDIO_def] \\ xpull) >>
+  reverse (Cases_on`consistentFS fs`) >- (
+    fs [STDIO_def,IOFS_def,wfFS_def,consistentFS_def]
+    \\ xpull \\ metis_tac[]) >>
+  xlet`(POSTv sv. &OPTION_TYPE (LIST_TYPE (LIST_TYPE (SUM_TYPE STRING_TYPE NUM)))
+            (if inFS_fname fs f then
+               SOME(MAP (MAP tokenize_num o tokens blanks) (all_lines fs f))
+             else NONE) sv * STDIO fs)`
+  >- (
+    xapp_spec b_inputAllTokensFrom_spec_specialize >>
+    xsimpl>>
+    fs[FILENAME_def,validArg_def,blanks_v_thm]>>
+    EVAL_TAC)>>
+  simp[get_graph_def]>>
+  reverse IF_CASES_TAC>>fs[OPTION_TYPE_def]>>xmatch
+  >- (
+    xlet_autop>>
+    xcon>>xsimpl>>
+    simp[SUM_TYPE_def]>>metis_tac[])>>
+  xlet_autop>>
+  `toks_num = (MAP tokenize_num ∘ tokens blanks)` by
+    metis_tac[toks_num_def,ETA_AX,o_DEF]>>
+  Cases_on`parse_lad (all_lines fs f)`>>
+  gvs[parse_lad_def,OPTION_TYPE_def]
+  >- (
+    xmatch >>
+    xlet_autop>>
+    xcon>>xsimpl>>
+    simp[SUM_TYPE_def]>>metis_tac[])>>
+  xmatch>>
+  xlet_autop>>
+  fs[check_good_graph_iff]>>
+  xif
+  >- (
+    xcon>>xsimpl>>
+    simp[SUM_TYPE_def])>>
+  rpt xlet_autop>>
+  xcon>>xsimpl>>
+  simp[SUM_TYPE_def]>>
+  metis_tac[]
+QED
+
+(* The encoder *)
+val _ = translate has_mapping_def;
+val _ = translate all_has_mapping_def;
+val _ = translate one_one_def;
+val _ = translate all_one_one_def;
+val _ = translate lookup_def;
+val _ = translate graph_basicTheory.neighbours_def;
+
+Theorem is_edge_compute:
+  is_edge e a b =
+  case lookup a e of NONE => F
+  | SOME ns => MEMBER b ns
+Proof
+  simp[graph_basicTheory.is_edge_def]>>
+  every_case_tac>>metis_tac[MEMBER_INTRO]
+QED
+
+val _ = translate is_edge_compute;
+
+val _ = translate edge_map_def;
+
+val _ = translate COUNT_LIST_AUX_def;
+val _ = translate COUNT_LIST_compute;
+val _ = translate (graph_basicTheory.not_neighbours_def |> SIMP_RULE std_ss [MEMBER_INTRO]);
+val _ = translate not_edge_map_def;
+val _ = translate all_full_edge_map_def;
+
+val _ = translate encode_base_def;
+
+val _ = translate pbcTheory.negate_def;
+val _ = translate iff_and_def;
+val _ = translate iff_or_def;
+val _ = translate walk_base_def;
+val _ = translate walk_aux_def;
+val _ = translate walk_ind_def;
+val _ = translate walk_k_def;
+
+(* TODO: use PRECONDITION *)
+Definition log2_def:
+  log2 n =
+  if n < 2 then 0:num
+  else (log2 (n DIV 2))+1
+End
+
+Theorem LOG2_log2:
+  ∀n.
+  n ≥ 1 ⇒
+  LOG 2 n = log2 n
+Proof
+  ho_match_mp_tac log2_ind>>rw[]>>
+  simp[Once log2_def]>>rw[]
+  >- (
+    `n=1`by fs[]>>
+    rw[])>>
+  REWRITE_TAC[Once numeral_bitTheory.LOG_compute]>>
+  fs[ADD1]>>
+  first_x_assum match_mp_tac>>
+  intLib.ARITH_TAC
+QED
+
+Theorem encode_connected_thm:
+  encode_connected (vp,ep) =
+  if vp = 0 then []
+  else
+  let k = log2 (vp*2-1) in
+  walk_k (vp,ep) k ++
+  FLAT (GENLIST (λf.
+    FLAT (GENLIST (λg.
+      if f < g then
+        [(GreaterEqual, [(1, Pos(Unmapped f));(1, Pos(Unmapped g));(1, Pos(Walk f g k))], 1)]
+      else []) vp)) vp)
+Proof
+  rw[encode_connected_def]>>
+  DEP_REWRITE_TAC [LOG2_log2]>>
+  fs[]
+QED
+
+val _ = translate log2_def;
+val _ = translate (encode_connected_thm);
+val _ = translate encode_def;
+
+(* Translate the string converter *)
+val res = translate enc_string_def;
+
+val _ = translate pbcTheory.map_obj_def;
+val _ = translate unmapped_obj_def;
+
+val _ = translate full_encode_def;
+
+(* parse input from f1 f2 and run encoder into pbc *)
+val parse_and_enc = (append_prog o process_topdecs) `
+  fun parse_and_enc f1 f2 =
+  case parse_lad f1 of
+    Inl err => Inl err
+  | Inr gp =>
+  (case parse_lad f2 of
+    Inl err => Inl err
+  | Inr gt =>
+    Inr (fst gp, full_encode gp gt))`
+
+Theorem parse_and_enc_spec:
+  STRING_TYPE f1 f1v ∧
+  STRING_TYPE f2 f2v ∧
+  validArg f1 ∧
+  validArg f2 ∧
+  hasFreeFD fs
+  ⇒
+  app (p:'ffi ffi_proj) ^(fetch_v"parse_and_enc"(get_ml_prog_state()))
+    [f1v;f2v]
+    (STDIO fs)
+    (POSTv v.
+    STDIO fs *
+    & ∃res.
+       SUM_TYPE STRING_TYPE
+         (PAIR_TYPE NUM (PAIR_TYPE
+            (OPTION_TYPE (PAIR_TYPE
+              (LIST_TYPE (PAIR_TYPE INT (PBC_LIT_TYPE STRING_TYPE)))
+            INT))
+            (LIST_TYPE (PAIR_TYPE PBC_PBOP_TYPE (PAIR_TYPE (LIST_TYPE (PAIR_TYPE INT (PBC_LIT_TYPE STRING_TYPE))) INT)))
+            )) res v ∧
+       case res of
+        INL err =>
+          get_graph fs f1 = NONE ∨
+          get_graph fs f2 = NONE
+      | INR (n,objf) =>
+        ∃gp gt.
+        get_graph fs f1 = SOME gp ∧
+        get_graph fs f2 = SOME gt ∧
+        full_encode gp gt = objf ∧
+        FST gp = n)
+Proof
+  rw[]>>
+  xcf"parse_and_enc"(get_ml_prog_state())>>
+  xlet_autop>>
+  every_case_tac>>fs[SUM_TYPE_def]>>xmatch
+  >- (
+    xcon>>xsimpl>>
+    qexists_tac`INL err`>>simp[SUM_TYPE_def])>>
+  xlet_autop>>
+  every_case_tac>>fs[SUM_TYPE_def]>>xmatch
+  >- (
+    xcon>>xsimpl>>
+    qexists_tac`INL err`>>simp[SUM_TYPE_def])>>
+  rpt xlet_autop>>
+  xcon>>xsimpl >>
+  rename1`_ (full_encode gpp gtt)`>>
+  qexists_tac`INR (FST gpp,full_encode gpp gtt)`>>
+  simp[SUM_TYPE_def,PAIR_TYPE_def]
+QED
+
+(* Printing answer *)
+Definition int_inf_to_string_def:
+  (int_inf_to_string NONE = strlit "INF") ∧
+  (int_inf_to_string (SOME (i:int)) =
+    toString i)
+End
+
+Definition print_mcis_bound_def:
+  print_mcis_bound (lbg:num option,ubg:num) =
+  case lbg of
+    NONE =>
+    strlit "s VERIFIED MCIS BOUNDS " ^ strlit "|MCIS| <= " ^ toString ubg ^ strlit"\n"
+  | SOME l =>
+    strlit "s VERIFIED MCIS BOUNDS " ^ toString l ^ strlit " <= |MCIS| <= " ^ toString ubg ^ strlit"\n"
+End
+
+Definition mcis_sem_def:
+  mcis_sem gp gt (lbg,ubg) ⇔
+  (∀f vs.
+    injective_partial_map f vs gp gt ∧
+    connected_subgraph vs (SND gp) ⇒
+    CARD vs ≤ ubg) ∧
+  case lbg of NONE => T
+  | SOME lb =>
+    ∃f vs.
+      injective_partial_map f vs gp gt ∧
+      connected_subgraph vs (SND gp) ∧
+      lb ≤ CARD vs
+End
+
+Definition check_unsat_3_sem_def:
+  check_unsat_3_sem fs f1 f2 out ⇔
+  (out ≠ strlit"" ⇒
+  ∃gp gt bounds.
+    get_graph fs f1 = SOME gp ∧
+    get_graph fs f2 = SOME gt ∧
+    out = print_mcis_bound bounds ∧
+    mcis_sem gp gt bounds)
+End
+
+Definition map_concl_to_string_def:
+  (map_concl_to_string n (INL s) = (INL s)) ∧
+  (map_concl_to_string n (INR c) =
+    case conv_concl n c of
+      SOME bounds => INR (print_mcis_bound bounds)
+    | NONE => INL (strlit "c Unexpected conclusion for MCIS problem.\n"))
+End
+
+val res = translate conv_concl_def;
+
+val conv_concl_side = Q.prove(
+  `∀x y. conv_concl_side x y <=> T`,
+  EVAL_TAC>>
+  rw[]>>
+  intLib.ARITH_TAC) |> update_precondition;
+
+val res = translate print_mcis_bound_def;
+val res = translate map_concl_to_string_def;
+
+val check_unsat_3 = (append_prog o process_topdecs) `
+  fun check_unsat_3 f1 f2 f3 =
+  case parse_and_enc f1 f2 of
+    Inl err => TextIO.output TextIO.stdErr err
+  | Inr (n,objf) =>
+    (case
+      map_concl_to_string n
+        (check_unsat_top_norm objf f3) of
+      Inl err => TextIO.output TextIO.stdErr err
+    | Inr s => TextIO.print s)`
+
+Theorem check_unsat_3_spec:
+  STRING_TYPE f1 f1v ∧ validArg f1 ∧
+  STRING_TYPE f2 f2v ∧ validArg f2 ∧
+  STRING_TYPE f3 f3v ∧ validArg f3 ∧
+  hasFreeFD fs
+  ⇒
+  app (p:'ffi ffi_proj) ^(fetch_v"check_unsat_3"(get_ml_prog_state()))
+    [f1v; f2v; f3v]
+    (STDIO fs)
+    (POSTv uv. &UNIT_TYPE () uv *
+    SEP_EXISTS out err.
+      STDIO (add_stdout (add_stderr fs err) out) *
+      &(check_unsat_3_sem fs f1 f2 out))
+Proof
+  rw[check_unsat_3_sem_def]>>
+  xcf "check_unsat_3" (get_ml_prog_state ())>>
+  reverse (Cases_on `STD_streams fs`) >- (fs [TextIOProofTheory.STDIO_def] \\ xpull) >>
+  xlet_autop>>
+  Cases_on`res`>>fs[SUM_TYPE_def]
+  >- (
+    xmatch>>
+    xapp_spec output_stderr_spec \\ xsimpl>>
+    asm_exists_tac>>xsimpl>>
+    qexists_tac`emp`>>xsimpl>>
+    qexists_tac`fs`>>xsimpl>>
+    rw[]>>
+    qexists_tac`x`>>xsimpl>>rw[]>>
+    fs[STD_streams_add_stderr, STD_streams_stdout,add_stdo_nil]>>
+    xsimpl)
+  >- (
+    xmatch>>
+    xapp_spec output_stderr_spec \\ xsimpl>>
+    asm_exists_tac>>xsimpl>>
+    qexists_tac`emp`>>xsimpl>>
+    qexists_tac`fs`>>xsimpl>>
+    rw[]>>
+    qexists_tac`x`>>xsimpl>>rw[]>>
+    fs[STD_streams_add_stderr, STD_streams_stdout,add_stdo_nil]>>
+    xsimpl)>>
+  Cases_on`y`>>fs[PAIR_TYPE_def]>>
+  xmatch>>
+  xlet_auto
+  >- (
+    xsimpl>>
+    fs[validArg_def]>>
+    metis_tac[])>>
+  xlet_autop>>
+  every_case_tac>>gvs[SUM_TYPE_def]
+  >- (
+    fs[map_concl_to_string_def,SUM_TYPE_def]>>
+    xmatch>>
+    xapp_spec output_stderr_spec \\ xsimpl>>
+    asm_exists_tac>>xsimpl>>
+    qexists_tac`emp`>>xsimpl>>
+    qexists_tac`fs`>>xsimpl>>
+    rw[]>>
+    qexists_tac`strlit ""`>>
+    rename1`add_stderr _ err`>>
+    qexists_tac`err`>>xsimpl>>rw[]>>
+    fs[STD_streams_add_stderr, STD_streams_stdout,add_stdo_nil]>>
+    xsimpl)>>
+  fs[map_concl_to_string_def]>>
+  every_case_tac>>fs[SUM_TYPE_def]>>xmatch
+  >- (
+    xapp_spec output_stderr_spec \\ xsimpl>>
+    asm_exists_tac>>xsimpl>>
+    qexists_tac`emp`>>xsimpl>>
+    qexists_tac`fs`>>xsimpl>>
+    rw[]>>
+    qexists_tac`strlit ""`>>
+    rename1`add_stderr _ err`>>
+    qexists_tac`err`>>xsimpl>>rw[]>>
+    fs[STD_streams_add_stderr, STD_streams_stdout,add_stdo_nil]>>
+    xsimpl)
+  >- (
+    xapp>>xsimpl>>
+    asm_exists_tac>>simp[]>>
+    qexists_tac`emp`>>qexists_tac`fs`>>xsimpl>>
+    rw[]>>
+    qexists_tac`print_mcis_bound x`>>simp[]>>
+    qexists_tac`strlit ""`>>
+    rw[]>>simp[STD_streams_stderr,add_stdo_nil]>>
+    xsimpl>>
+    (drule_at Any) full_encode_sem_concl>>
+    fs[]>>
+    Cases_on`x`>> disch_then (drule_at Any)>>
+    disch_then(qspec_then`gt'` mp_tac)>>
+    impl_tac>-
+      fs[get_graph_def,AllCaseEqs()]>>
+    rw[]>>
+    qexists_tac`(q,r)`>>
+    simp[mcis_sem_def]>>
+    metis_tac[])
+QED
+
+Definition check_unsat_2_sem_def:
+  check_unsat_2_sem fs f1 f2 out ⇔
+  case get_graph fs f1 of
+    NONE => out = strlit ""
+  | SOME gpp =>
+  case get_graph fs f2 of
+    NONE => out = strlit ""
+  | SOME gtt =>
+    out = concat (print_pbf (full_encode gpp gtt))
+End
+
+val check_unsat_2 = (append_prog o process_topdecs) `
+  fun check_unsat_2 f1 f2 =
+  case parse_and_enc f1 f2 of
+    Inl err => TextIO.output TextIO.stdErr err
+  | Inr (n,objf) =>
+    TextIO.print_list (print_pbf objf)`
+
+Theorem check_unsat_2_spec:
+  STRING_TYPE f1 f1v ∧ validArg f1 ∧
+  STRING_TYPE f2 f2v ∧ validArg f2 ∧
+  hasFreeFD fs
+  ⇒
+  app (p:'ffi ffi_proj) ^(fetch_v"check_unsat_2"(get_ml_prog_state()))
+    [f1v;f2v]
+    (STDIO fs)
+    (POSTv uv. &UNIT_TYPE () uv *
+    SEP_EXISTS out err.
+      STDIO (add_stdout (add_stderr fs err) out) *
+      &(check_unsat_2_sem fs f1 f2 out))
+Proof
+  rw[check_unsat_2_sem_def]>>
+  xcf "check_unsat_2" (get_ml_prog_state ())>>
+  reverse (Cases_on `STD_streams fs`) >- (fs [TextIOProofTheory.STDIO_def] \\ xpull) >>
+  xlet_autop>>
+  Cases_on`res`>>fs[SUM_TYPE_def]
+  >- (
+    xmatch>>
+    xapp_spec output_stderr_spec \\ xsimpl>>
+    asm_exists_tac>>xsimpl>>
+    qexists_tac`emp`>>qexists_tac`fs`>>xsimpl>>
+    fs[STD_streams_add_stderr, STD_streams_stdout,add_stdo_nil]>>
+    rw[]>>
+    qexists_tac`x`>>xsimpl)
+  >- (
+    xmatch>>
+    xapp_spec output_stderr_spec \\ xsimpl>>
+    asm_exists_tac>>xsimpl>>
+    qexists_tac`emp`>>qexists_tac`fs`>>xsimpl>>
+    every_case_tac>>xsimpl>>
+    fs[STD_streams_add_stderr, STD_streams_stdout,add_stdo_nil]>>
+    rw[]>>
+    qexists_tac`x`>>xsimpl)>>
+  Cases_on`y`>>gvs[PAIR_TYPE_def]>>
+  xmatch>>
+  xlet_autop>>
+  xapp_spec print_list_spec>>xsimpl>>
+  asm_exists_tac>>xsimpl>>
+  qexists_tac`emp`>>qexists_tac`fs`>>xsimpl>>
+  rw[]>>
+  qexists_tac`strlit ""`>>
+  simp[STD_streams_stderr,add_stdo_nil]>>
+  xsimpl
+QED
+
+Definition usage_string_def:
+  usage_string = strlit "Usage: cake_mcis <LAD file (pattern)> <LAD file (target)> <optional: PB proof file>\n"
+End
+
+val r = translate usage_string_def;
+
+val main = (append_prog o process_topdecs) `
+  fun main u =
+  case CommandLine.arguments () of
+    [f1,f2] => check_unsat_2 f1 f2
+  | [f1,f2,f3] => check_unsat_3 f1 f2 f3
+  | _ => TextIO.output TextIO.stdErr usage_string`
+
+Definition main_sem_def:
+  main_sem fs cl out =
+  if LENGTH cl = 3 then
+    check_unsat_2_sem fs (EL 1 cl) (EL 2 cl) out
+  else if LENGTH cl = 4 then
+    check_unsat_3_sem fs (EL 1 cl) (EL 2 cl) out
+  else out = strlit ""
+End
+
+Theorem STDIO_refl:
+  STDIO A ==>>
+  STDIO A * GC
+Proof
+  xsimpl
+QED
+
+Theorem main_spec:
+  hasFreeFD fs
+  ⇒
+  app (p:'ffi ffi_proj) ^(fetch_v"main"(get_ml_prog_state()))
+    [Conv NONE []]
+    (COMMANDLINE cl * STDIO fs)
+    (POSTv uv. &UNIT_TYPE () uv *
+    COMMANDLINE cl *
+    SEP_EXISTS out err.
+      STDIO (add_stdout (add_stderr fs err) out) *
+      &(main_sem fs cl out))
+Proof
+  rw[main_sem_def]>>
+  xcf"main"(get_ml_prog_state())>>
+  reverse (Cases_on `STD_streams fs`) >- (fs [TextIOProofTheory.STDIO_def] \\ xpull) >>
+  reverse(Cases_on`wfcl cl`) >- (fs[COMMANDLINE_def] \\ xpull)>>
+  rpt xlet_autop >>
+  Cases_on `cl` >- fs[wfcl_def] >>
+  Cases_on`t`>>fs[LIST_TYPE_def]
+  >- (
+    xmatch>>
+    xapp_spec output_stderr_spec \\ xsimpl>>
+    rename1`COMMANDLINE cl`>>
+    qexists_tac`COMMANDLINE cl`>>xsimpl>>
+    qexists_tac `usage_string` >>
+    simp [theorem "usage_string_v_thm"] >>
+    qexists_tac`fs`>>xsimpl>>
+    rw[]>>
+    fs[STD_streams_add_stderr, STD_streams_stdout,add_stdo_nil]>>
+    metis_tac[STDIO_refl])>>
+  Cases_on`t'`>>fs[LIST_TYPE_def]
+  >- (
+    xmatch>>
+    xapp_spec output_stderr_spec \\ xsimpl>>
+    rename1`COMMANDLINE cl`>>
+    qexists_tac`COMMANDLINE cl`>>xsimpl>>
+    qexists_tac `usage_string` >>
+    simp [theorem "usage_string_v_thm"] >>
+    qexists_tac`fs`>>xsimpl>>
+    rw[]>>
+    fs[STD_streams_add_stderr, STD_streams_stdout,add_stdo_nil]>>
+    metis_tac[STDIO_refl])>>
+  Cases_on`t`>>fs[LIST_TYPE_def]
+  >- (
+    xmatch>>
+    xapp>>rw[]>>
+    rpt(first_x_assum (irule_at Any)>>xsimpl)>>
+    fs[wfcl_def]>>
+    rw[]>>metis_tac[STDIO_refl])>>
+  Cases_on`t'`>>fs[LIST_TYPE_def]
+  >- (
+    xmatch>>
+    xapp>>rw[]>>
+    rpt(first_x_assum (irule_at Any)>>xsimpl)>>
+    fs[wfcl_def]>>
+    rw[]>>metis_tac[STDIO_refl])>>
+  xmatch>>
+  xapp_spec output_stderr_spec \\ xsimpl>>
+  rename1`COMMANDLINE cl`>>
+  qexists_tac`COMMANDLINE cl`>>xsimpl>>
+  qexists_tac `usage_string` >>
+  simp [theorem "usage_string_v_thm"] >>
+  qexists_tac`fs`>>xsimpl>>
+  rw[]>>
+  fs[STD_streams_add_stderr, STD_streams_stdout,add_stdo_nil]>>
+  metis_tac[STDIO_refl]
+QED
+
+Theorem main_whole_prog_spec2:
+   hasFreeFD fs ⇒
+   whole_prog_spec2 main_v cl fs NONE
+     (λfs'. ∃out err.
+        fs' = add_stdout (add_stderr fs err) out ∧
+        main_sem fs cl out)
+Proof
+  rw[basis_ffiTheory.whole_prog_spec2_def]
+  \\ match_mp_tac (MP_CANON (DISCH_ALL (MATCH_MP app_wgframe (UNDISCH main_spec))))
+  \\ xsimpl
+  \\ rw[PULL_EXISTS]
+  \\ qexists_tac`add_stdout (add_stderr fs x') x`
+  \\ xsimpl
+  \\ qexists_tac`x`
+  \\ qexists_tac`x'`
+  \\ xsimpl
+  \\ simp[GSYM add_stdo_with_numchars,with_same_numchars]
+QED
+
+local
+
+val name = "main"
+val (sem_thm,prog_tm) =
+  whole_prog_thm (get_ml_prog_state()) name (UNDISCH main_whole_prog_spec2)
+val main_prog_def = Define`main_prog = ^prog_tm`;
+
+in
+
+Theorem main_semantics =
+  sem_thm
+  |> REWRITE_RULE[GSYM main_prog_def]
+  |> DISCH_ALL
+  |> SIMP_RULE(srw_ss())[GSYM CONJ_ASSOC,AND_IMP_INTRO];
+
+end
+
+val _ = export_theory();
